loadHalf/Word/Double_spec

src/ListMemory.v
@@ -61,6 +61,8 @@ Local Ltac wrap L :=
   try apply wordToNat_neq1;
   (congruence || momega || idtac).    
 
+Definition TODO{T: Type}: T. Admitted.
+
 Instance mem_is_Memory(w: nat): Memory (mem w) w := {|
   memSize     := mem_size;
   loadByte    := read_byte;
@@ -85,4 +87,10 @@ Instance mem_is_Memory(w: nat): Memory (mem w) w := {|
 - wrap ListMemoryNatAddr.write_read_double_eq.
 - wrap ListMemoryNatAddr.write_read_double_ne.
 - wrap ListMemoryNatAddr.write_double_preserves_mem_size.
+- intros. unfold read_half. unfold ListMemoryNatAddr.read_half.
+  unfold read_byte.
+  unfold valid_addr, mem_size in *.
+  apply TODO. (* we need word lemmas not yet in Word.v *)
+- apply TODO.
+- apply TODO.
 Defined.
